Change InternalNode representation to array

xi-rope.dfy
@@ -9,7 +9,6 @@ module Rope {
   class Rope {
     ghost var Repr: set<Rope>
     ghost var Content: seq<string>
-    ghost var HasParent: bool
 
     var val: Node
     var len: int
@@ -24,14 +23,12 @@ module Rope {
       height := 0;
       Repr := {this};
       Content := [""];
-      HasParent := false;
     }
 
 
     constructor FromNodes(nodes: seq<Rope>)
-//      requires forall c: Rope :: c in nodes ==> c.ValidLen()
-//      requires |nodes| >= MIN_CHILDREN && |nodes| <= MAX_CHILDREN
-//      ensures match this.val case Leaf(c) => true case InternalNode(children) => forall c: Rope :: c in children ==> c.HasParent
+      requires forall c: Rope :: c in nodes ==> c.Valid() && c.ValidLen()
+      requires |nodes| >= MIN_CHILDREN && |nodes| <= MAX_CHILDREN
 //      ensures Valid()
 //      ensures ValidLen()
       modifies nodes
@@ -39,9 +36,8 @@ module Rope {
       var i := 0;
       Content := [];
       Repr := {};
-      HasParent := false;
       var totalLen := 0;
-      var tmpNodes: seq<Rope> := [];
+      val := InternalNode(nodes);
 
       while i < |nodes|
       {
@@ -49,21 +45,14 @@ module Rope {
         Content := Content + nodes[i].Content;
         var c := new Rope.Init();
         c.len := nodes[i].len;
-        c.HasParent := true;
         c.Content := nodes[i].Content;
         c.Repr := c.Repr + nodes[i].Repr - {nodes[i]};
-        Repr := Repr + c.Repr;
-
-        tmpNodes := tmpNodes + [c];
-
-//        nodes[i].HasParent := true;
-//        Repr := Repr + nodes[i].Repr;
+        Repr := Repr + nodes[i].Repr;
 
         i := i + 1;
       }
 
       len := totalLen;
-      val := InternalNode(tmpNodes);
       Repr := Repr + {this};
     }
 
@@ -93,6 +82,26 @@ module Rope {
       case InternalNode(children) => this.len == this.Len() && this.len >= 0 && forall c: Rope :: c in children ==> c.len <= this.len && c.ValidLen()
     }
 
+    predicate ValidNonRoot()
+      reads this, Repr
+      requires MAX_LEAF_LEN >= MIN_LEAF_LEN
+      requires MIN_CHILDREN <= MAX_CHILDREN && MIN_CHILDREN >= 2
+    {
+      this in Repr &&
+      (
+        match this.val
+        case Leaf(v) => |v| <= MAX_LEAF_LEN && Content == [v] && height == 0
+        case InternalNode(children) =>
+          height >= 0 &&
+          |children| >= MIN_CHILDREN &&
+          |children| <= MAX_CHILDREN &&
+          forall c: Rope :: c in children ==> 
+            c in Repr && this !in c.Repr && c.Repr < Repr && c.ValidNonRoot() &&
+            c.height == height - 1 && c.Content <= Content &&
+            forall cont: string :: cont in c.Content ==> cont in this.Content
+      )
+    }
+    
     predicate Valid()
       reads this, Repr
       requires MAX_LEAF_LEN >= MIN_LEAF_LEN
@@ -104,16 +113,12 @@ module Rope {
         case Leaf(v) => |v| <= MAX_LEAF_LEN && Content == [v] && height == 0
         case InternalNode(children) =>
           height >= 0 &&
-          (HasParent ==>
-            |children| >= MIN_CHILDREN &&
-            |children| <= MAX_CHILDREN &&
-            forall c: Rope :: c in children ==> c in Repr && this !in c.Repr && c.Repr < Repr && c.Valid() && c.height == height - 1 && c.Content <= Content && forall cont: string :: cont in c.Content ==> cont in this.Content
-          ) &&
-          (!HasParent ==>
-            |children| >= 2 &&
-            |children| <= MAX_CHILDREN &&
-            forall c: Rope :: c in children ==> c in Repr && this !in c.Repr && c.Repr < Repr && c.Valid() && c.height == height - 1 && c.Content <= Content && forall cont: string :: cont in c.Content ==> cont in this.Content
-          )
+          |children| >= 2 &&
+          |children| <= MAX_CHILDREN &&
+          forall c: Rope :: c in children ==> 
+            c in Repr && this !in c.Repr && c.Repr < Repr &&
+            c.ValidNonRoot() && c.height == height - 1 && c.Content <= Content &&
+            forall cont: string :: cont in c.Content ==> cont in this.Content
       )
     }
 
@@ -198,6 +203,139 @@ module Rope {
 
               slice := finalSlice;
           }
+    }
+  }
+}
+
+
+
+-----------------
+
+
+module Rope {
+  const MAX_CHILDREN: nat := 4
+  const MIN_CHILDREN: nat := 2
+  const MAX_LEAF_LEN: nat := 10
+  const MIN_LEAF_LEN: nat := 2   // minimum size requirement when splitting
+
+  datatype Node = Leaf(value: string) | InternalNode(children: array<Rope>)
+
+  class Rope {
+    ghost var Repr: set<Rope>
+    ghost var Content: seq<string>
+
+    var val: Node
+    var len: int
+    var height: int
+
+    constructor Init()
+//      ensures Valid()
+//      ensures ValidLen()
+    {
+      val := Leaf("");
+      len := 0;
+      height := 0;
+      Repr := {this};
+      Content := [""];
+    }
+
+
+    constructor FromNodes(nodes: array<Rope>)
+//      requires forall c: Rope :: c in nodes ==> c.Valid() && c.ValidLen()
+     // requires |nodes| >= MIN_CHILDREN && |nodes| <= MAX_CHILDREN
+      
+      //ensures Valid()
+      //ensures ValidLen()
+      modifies nodes
+    {
+      var i := 0;
+      Content := [];
+      Repr := {};
+      var totalLen := 0;
+      var r := new Rope.Init();
+      var tmp := new Rope[nodes.Length](_ => r);
+      
+      while i < nodes.Length
+      {
+        tmp[i] := nodes[i];
+        totalLen := totalLen + tmp[i].len;
+        Content := Content + tmp[i].Content;
+        Repr := Repr + tmp[i].Repr;
+
+        i := i + 1;
+      }
+
+      val := InternalNode(tmp);
+      len := totalLen;
+      Repr := Repr + {this};
+    }
+  
+
+    function ContentLen(c: seq<string>): int
+      decreases |c|
+    {
+      if |c| == 0 then 0
+      else |c[0]| + ContentLen(c[1..])
+    }
+
+    function Len(): int
+      requires Valid()
+      reads *
+      decreases Repr
+    {
+      match this.val
+      case Leaf(v) => |v|
+      case InternalNode(children) => ContentLen(this.Content)
+    }
+
+    predicate ValidLen()
+      requires Valid()
+      reads *
+      decreases Repr
+    {
+      match this.val
+      case Leaf(v) => this.len == |v| && ContentLen(this.Content) == |v| && |Content| == 1
+      case InternalNode(children) => this.len == this.Len() && this.len >= 0 && forall k: int :: 0 <= k < children.Length ==> children[k].len <= this.len && children[k].ValidLen()
+    }
+
+    predicate ValidNonRoot()
+      reads *
+      requires MAX_LEAF_LEN >= MIN_LEAF_LEN
+      requires MIN_CHILDREN <= MAX_CHILDREN && MIN_CHILDREN >= 2
+      decreases Repr
+    {
+      this in Repr &&
+      (
+        match this.val
+        case Leaf(v) => |v| <= MAX_LEAF_LEN && Content == [v] && height == 0
+        case InternalNode(children) =>
+          height >= 0 &&
+          children.Length >= MIN_CHILDREN &&
+          children.Length <= MAX_CHILDREN &&
+          forall k: int :: 0 <= k < children.Length ==>
+            children[k] in Repr && this !in children[k].Repr && children[k].Repr < Repr && children[k].ValidNonRoot() &&
+            children[k].height == height - 1 && children[k].Content <= Content &&
+            forall cont: string :: cont in children[k].Content ==> cont in this.Content
+      )
+    }
+    
+    predicate Valid()
+      reads *
+      requires MAX_LEAF_LEN >= MIN_LEAF_LEN
+      requires MIN_CHILDREN <= MAX_CHILDREN && MIN_CHILDREN >= 2
+    {
+      this in Repr &&
+      (
+        match this.val
+        case Leaf(v) => |v| <= MAX_LEAF_LEN && Content == [v] && height == 0
+        case InternalNode(children) =>
+          height >= 0 &&
+          children.Length <= MAX_CHILDREN &&
+          forall k: int :: 0 <= k < children.Length ==>
+            children[k] in Repr && this !in children[k].Repr && children[k].Repr < Repr && children[k].ValidNonRoot() &&
+            children[k].height == height - 1 && children[k].Content <= Content &&
+            forall cont: string :: cont in children[k].Content ==> cont in this.Content
+      )
     }
   }
 }
