rope.dfy
@@ -1,344 +1,347 @@
-datatype Node = Leaf(value: string) | InternalNode(left: Rope?, right: Rope?)
+module Rope {
+  datatype Node = Leaf(value: string) | InternalNode(left: Rope?, right: Rope?)
 
-class Rope {
-  ghost var Repr: set<object>
+  class Rope {
 
-  var len: int
-  var val: Node
-
-  constructor Init()
-  ensures Valid()
-  ensures ValidLen()
-  {
-    val := InternalNode(null, null);
-    len := 0;
-    Repr := {this};
-  }
-
-  function method Len(): int
-    requires Valid()
-    reads Repr
-    decreases Repr
-  {
-    match this.val
-    case Leaf(v) => |v|
-    case InternalNode(left, right) =>
-      if left != null && right != null then left.Len() + right.Len()
-      else if left == null && right != null then right.Len()
-      else if left != null && right == null then left.Len()
-      else if left == null && right == null then 0
-      else 0
-  }
-
-  predicate ValidLen()
-    requires Valid()
-    reads this, Repr
-  {
-    match this.val
-    case Leaf(v) => this.len == |v|
-    case InternalNode(left, right) =>
-      (left != null ==> this.len == left.Len() && left.ValidLen()) &&
-      (left == null ==> this.len == 0) &&
-      (right != null ==> right.ValidLen())
-  }
-
-  predicate Valid()
-    reads this, Repr
-  {
-    this in Repr &&
-    (
-      match this.val
-      case Leaf(v) => true
-      case InternalNode(left, right) =>
-        (left != null ==>
-          left in this.Repr && this.Repr >= left.Repr && this !in left.Repr && left.Valid()
-        ) &&
-        (right != null ==>
-          right in this.Repr && this.Repr >= right.Repr && this !in right.Repr && right.Valid()
-        )
-    )
-  }
-
-  function method Report(): string
-    requires Valid()
-    requires ValidLen()
-    reads Repr
-    decreases Repr
-    ensures |this.Report()| == this.Len()
-  {
-    if this.Len() == 0 then ""
-    else
-      match this.val
-      case Leaf(v) => v
-      case InternalNode(left, right) =>
-        if left != null && right != null then left.Report() + right.Report()
-        else if left == null && right != null then right.Report()
-        else if left != null && right == null then left.Report()
-        else if left == null && right == null then ""
-        else ""
-  }
-
-  method Delete(i: int, j: int) returns (newRope: Rope?)
-    requires Valid()
-    requires ValidLen()
-    ensures newRope != null ==> newRope.Valid()
-    ensures newRope != null ==> newRope.ValidLen()
-    ensures j < i ==> newRope == null
-    ensures i < 0 || i >= this.Len() || j < j || j >= this.Len() ==> newRope == null
-    //ensures i == 0 && j == this.Len() - 1 && newRope != null ==> newRope.len == 0
-    // todo: len
-  {
-    if i < 0 || j < 0 || i >= this.Len() || j >= this.Len() || i > j
-      {
-        newRope := null;
-      }
-    else
-      {
-        var newLeft, _ := this.Split(i);
-        var _, newRight := this.Split(j);
-
-        if newLeft == null
-          {
-            if newRight == null
-              {
-                newRope := new Rope.Init();
-              }
-            else
-              {
-                newRope := newRight;
-              }
-          }
-        else
-          {
-            if newRight == null
-              {
-                newRope := newLeft;
-              }
-            else
-              {
-                newRope := newLeft.Concat(newRight);
-              }
-          }
-      }
-  }
-
-  method Insert(i: int, s: string) returns (newRope: Rope?)
-    requires Valid()
-    requires ValidLen()
+    ghost var Repr: set<object>
+  
+    var len: int
+    var val: Node
+  
+    constructor Init()
     ensures Valid()
     ensures ValidLen()
-    ensures newRope != null ==> newRope.Valid()
-    ensures newRope != null ==> newRope.ValidLen()
-    ensures i < 0 || i >= this.Len() <==> newRope == null
-//    ensures newRope != null ==> newRope.Len() >= this.Len() [todo]
-  {
-    if i < 0
-      {
-        newRope := null;
-      }
-    else if i >= this.Len()
-      {
-        newRope := null;
-      }
-    else
-      {
-        var insertedLeaf := new Rope.Init();
-        insertedLeaf.val := Leaf(s);
-        insertedLeaf.len := |s|;
-
-        var leftSplit, rightSplit := this.Split(i);
-
-        if leftSplit == null
-          {
-            if rightSplit == null
+    {
+      val := InternalNode(null, null);
+      len := 0;
+      Repr := {this};
+    }
+  
+    function method Len(): int
+      requires Valid()
+      reads Repr
+      decreases Repr
+    {
+      match this.val
+      case Leaf(v) => |v|
+      case InternalNode(left, right) =>
+        if left != null && right != null then left.Len() + right.Len()
+        else if left == null && right != null then right.Len()
+        else if left != null && right == null then left.Len()
+        else if left == null && right == null then 0
+        else 0
+    }
+  
+    predicate ValidLen()
+      requires Valid()
+      reads this, Repr
+    {
+      match this.val
+      case Leaf(v) => this.len == |v|
+      case InternalNode(left, right) =>
+        (left != null ==> this.len == left.Len() && left.ValidLen()) &&
+        (left == null ==> this.len == 0) &&
+        (right != null ==> right.ValidLen())
+    }
+  
+    predicate Valid()
+      reads this, Repr
+    {
+      this in Repr &&
+      (
+        match this.val
+        case Leaf(v) => true
+        case InternalNode(left, right) =>
+          (left != null ==>
+            left in this.Repr && this.Repr >= left.Repr && this !in left.Repr && left.Valid()
+          ) &&
+          (right != null ==>
+            right in this.Repr && this.Repr >= right.Repr && this !in right.Repr && right.Valid()
+          )
+      )
+    }
+  
+    function method Report(): string
+      requires Valid()
+      requires ValidLen()
+      reads Repr
+      decreases Repr
+      ensures |this.Report()| == this.Len()
+    {
+      if this.Len() == 0 then ""
+      else
+        match this.val
+        case Leaf(v) => v
+        case InternalNode(left, right) =>
+          if left != null && right != null then left.Report() + right.Report()
+          else if left == null && right != null then right.Report()
+          else if left != null && right == null then left.Report()
+          else if left == null && right == null then ""
+          else ""
+    }
+  
+    method Delete(i: int, j: int) returns (newRope: Rope?)
+      requires Valid()
+      requires ValidLen()
+      ensures newRope != null ==> newRope.Valid()
+      ensures newRope != null ==> newRope.ValidLen()
+      ensures j < i ==> newRope == null
+      ensures i < 0 || i >= this.Len() || j < j || j >= this.Len() ==> newRope == null
+      //ensures i == 0 && j == this.Len() - 1 && newRope != null ==> newRope.len == 0
+      // todo: len
+    {
+      if i < 0 || j < 0 || i >= this.Len() || j >= this.Len() || i > j
+        {
+          newRope := null;
+        }
+      else
+        {
+          var newLeft, _ := this.Split(i);
+          var _, newRight := this.Split(j);
+  
+          if newLeft == null
+            {
+              if newRight == null
+                {
+                  newRope := new Rope.Init();
+                }
+              else
+                {
+                  newRope := newRight;
+                }
+            }
+          else
+            {
+              if newRight == null
+                {
+                  newRope := newLeft;
+                }
+              else
+                {
+                  newRope := newLeft.Concat(newRight);
+                }
+            }
+        }
+    }
+  
+    method Insert(i: int, s: string) returns (newRope: Rope?)
+      requires Valid()
+      requires ValidLen()
+      ensures Valid()
+      ensures ValidLen()
+      ensures newRope != null ==> newRope.Valid()
+      ensures newRope != null ==> newRope.ValidLen()
+      ensures i < 0 || i >= this.Len() <==> newRope == null
+  //    ensures newRope != null ==> newRope.Len() >= this.Len() [todo]
+    {
+      if i < 0
+        {
+          newRope := null;
+        }
+      else if i >= this.Len()
+        {
+          newRope := null;
+        }
+      else
+        {
+          var insertedLeaf := new Rope.Init();
+          insertedLeaf.val := Leaf(s);
+          insertedLeaf.len := |s|;
+  
+          var leftSplit, rightSplit := this.Split(i);
+  
+          if leftSplit == null
+            {
+              if rightSplit == null
+                {
+                  newRope := insertedLeaf;
+                }
+              else
+                {
+                  newRope := insertedLeaf.Concat(rightSplit);
+                }
+            }
+          else
+            {
+              var leftConcat := leftSplit.Concat(insertedLeaf);
+  
+              if rightSplit != null
+                {
+                  newRope := leftConcat.Concat(rightSplit);
+                }
+              else
+                {
+                  newRope := leftConcat;
+                }
+            }
+        }
+    }
+  
+    method Split(i: int) returns (leftSplit: Rope?, rightSplit: Rope?)
+      requires Valid()
+      requires ValidLen()
+      ensures leftSplit != null ==> leftSplit.Valid()
+      ensures rightSplit != null ==> rightSplit.Valid()
+      ensures rightSplit != null ==> rightSplit.ValidLen()
+      ensures leftSplit != null ==> leftSplit.ValidLen()
+      ensures i >= 0 && i < this.Len() ==> leftSplit != null || rightSplit != null
+      ensures i <= 0 ==> leftSplit == null
+      ensures i > 0 && i >= this.Len() ==> rightSplit == null
+      decreases Repr
+    {
+      if i <= 0
+        {
+          leftSplit := null;
+          rightSplit := this;
+        }
+      else if i >= this.Len()
+        {
+          leftSplit := this;
+          rightSplit := null;
+        }
+      else
+        {
+          match this.val
+          case Leaf(v) =>
+            var rightNode := new Rope.Init();
+            rightNode.val := Leaf(v[i..]);
+            rightNode.len := |v[i..]|;
+            rightNode.Repr := {rightNode};
+            rightSplit := rightNode;
+  
+            var leftLeaf := new Rope.Init();
+            leftLeaf.val := Leaf(v[0..i]);
+            leftLeaf.len := |v[0..i]|;
+            leftLeaf.Repr := {leftLeaf};
+  
+            var leftNode := new Rope.Init();
+            leftNode.val := InternalNode(leftLeaf, null);
+            leftNode.Repr := {leftNode, leftLeaf};
+            leftNode.len := leftLeaf.Len();
+            leftSplit := leftNode;
+  
+          case InternalNode(left, right) =>
+            if this.len >= i
               {
-                newRope := insertedLeaf;
+                var postLeft, postRight := left.Split(i);
+  
+                if postRight != null
+                  {
+                    var rightParent := new Rope.Init();
+                    rightParent.val := InternalNode(postRight, right);
+                    rightParent.len := postRight.Len();
+  
+                    if right != null
+                      {
+                        rightParent.Repr := rightParent.Repr + postRight.Repr + right.Repr;
+                      }
+                    else
+                      {
+                        rightParent.Repr := rightParent.Repr + postRight.Repr;
+                      }
+  
+                    rightSplit := rightParent;
+                  }
+               else
+                  {
+                     rightSplit := right;
+                  }
+  
+                var leftNode := new Rope.Init();
+                leftNode.val := InternalNode(postLeft, null);
+  
+                if postLeft != null
+                  {
+                    leftNode.Repr := leftNode.Repr + postLeft.Repr;
+                    leftNode.len := postLeft.Len();
+                  }
+                else
+                  {
+                    leftNode.Repr := leftNode.Repr;
+                    leftNode.len := 0;
+                  }
+  
+                leftSplit := leftNode;
               }
             else
               {
-                newRope := insertedLeaf.Concat(rightSplit);
+                var postLeft, postRight := right.Split(i);
+  
+                var leftNode := new Rope.Init();
+                leftNode.val := InternalNode(left, postLeft);
+                leftNode.len := 0;
+  
+                if postLeft != null
+                  {
+                    if left != null
+                      {
+                        leftNode.Repr := leftNode.Repr + left.Repr + postLeft.Repr;
+                        leftNode.len := left.Len();
+                      }
+                    else
+                      {
+                        leftNode.Repr := leftNode.Repr + postLeft.Repr;
+                      }
+                  }
+                else
+                  {
+                    if left != null
+                      {
+                        leftNode.Repr := leftNode.Repr + left.Repr;
+                        leftNode.len := left.Len();
+                      }
+                  }
+  
+                leftSplit := leftNode;
+  
+                rightSplit := postRight;
               }
+        }
+    }
+  
+    method Concat(rope: Rope) returns (concatenatedRope: Rope)
+      requires Valid()
+      requires ValidLen()
+      requires rope.Valid()
+      requires rope.ValidLen()
+      //requires this.Repr !! rope.Repr   // prevents cycles and concatenating the same rope with itself [todo?]
+      ensures concatenatedRope.Valid()
+      ensures concatenatedRope.ValidLen()
+    {
+      concatenatedRope := new Rope.Init();
+      concatenatedRope.val := InternalNode(this, rope);
+      concatenatedRope.len := this.Len();
+      concatenatedRope.Repr := concatenatedRope.Repr + this.Repr + rope.Repr;
+    }
+  
+    method Index(i: int) returns (charAtIndex: string)
+      requires Valid()
+      requires ValidLen()
+      ensures i >= 0 && this.Len() > i ==> charAtIndex != ""
+      //ensures i < 0 || this.Len() <= i ==> charAtIndex == ""
+      decreases Repr
+    {
+      match this.val
+      case Leaf(v) =>
+        if |v| <= i || i < 0
+          { charAtIndex := ""; }
+        else
+          { charAtIndex := [v[i]]; }
+      case InternalNode(left, right) =>
+        if this.len <= i
+          {
+            if right == null
+              { charAtIndex := ""; }
+            else
+              { charAtIndex := right.Index(i - this.len); }
           }
         else
           {
-            var leftConcat := leftSplit.Concat(insertedLeaf);
-
-            if rightSplit != null
-              {
-                newRope := leftConcat.Concat(rightSplit);
-              }
+            if left != null
+              { charAtIndex := left.Index(i); }
             else
-              {
-                newRope := leftConcat;
-              }
+              { charAtIndex := ""; }
           }
-      }
-  }
-
-  method Split(i: int) returns (leftSplit: Rope?, rightSplit: Rope?)
-    requires Valid()
-    requires ValidLen()
-    ensures leftSplit != null ==> leftSplit.Valid()
-    ensures rightSplit != null ==> rightSplit.Valid()
-    ensures rightSplit != null ==> rightSplit.ValidLen()
-    ensures leftSplit != null ==> leftSplit.ValidLen()
-    ensures i >= 0 && i < this.Len() ==> leftSplit != null || rightSplit != null
-    ensures i <= 0 ==> leftSplit == null
-    ensures i > 0 && i >= this.Len() ==> rightSplit == null
-    decreases Repr
-  {
-    if i <= 0
-      {
-        leftSplit := null;
-        rightSplit := this;
-      }
-    else if i >= this.Len()
-      {
-        leftSplit := this;
-        rightSplit := null;
-      }
-    else
-      {
-        match this.val
-        case Leaf(v) =>
-          var rightNode := new Rope.Init();
-          rightNode.val := Leaf(v[i..]);
-          rightNode.len := |v[i..]|;
-          rightNode.Repr := {rightNode};
-          rightSplit := rightNode;
-
-          var leftLeaf := new Rope.Init();
-          leftLeaf.val := Leaf(v[0..i]);
-          leftLeaf.len := |v[0..i]|;
-          leftLeaf.Repr := {leftLeaf};
-
-          var leftNode := new Rope.Init();
-          leftNode.val := InternalNode(leftLeaf, null);
-          leftNode.Repr := {leftNode, leftLeaf};
-          leftNode.len := leftLeaf.Len();
-          leftSplit := leftNode;
-
-        case InternalNode(left, right) =>
-          if this.len >= i
-            {
-              var postLeft, postRight := left.Split(i);
-
-              if postRight != null
-                {
-                  var rightParent := new Rope.Init();
-                  rightParent.val := InternalNode(postRight, right);
-                  rightParent.len := postRight.Len();
-
-                  if right != null
-                    {
-                      rightParent.Repr := rightParent.Repr + postRight.Repr + right.Repr;
-                    }
-                  else
-                    {
-                      rightParent.Repr := rightParent.Repr + postRight.Repr;
-                    }
-
-                  rightSplit := rightParent;
-                }
-             else
-                {
-                   rightSplit := right;
-                }
-
-              var leftNode := new Rope.Init();
-              leftNode.val := InternalNode(postLeft, null);
-
-              if postLeft != null
-                {
-                  leftNode.Repr := leftNode.Repr + postLeft.Repr;
-                  leftNode.len := postLeft.Len();
-                }
-              else
-                {
-                  leftNode.Repr := leftNode.Repr;
-                  leftNode.len := 0;
-                }
-
-              leftSplit := leftNode;
-            }
-          else
-            {
-              var postLeft, postRight := right.Split(i);
-
-              var leftNode := new Rope.Init();
-              leftNode.val := InternalNode(left, postLeft);
-              leftNode.len := 0;
-
-              if postLeft != null
-                {
-                  if left != null
-                    {
-                      leftNode.Repr := leftNode.Repr + left.Repr + postLeft.Repr;
-                      leftNode.len := left.Len();
-                    }
-                  else
-                    {
-                      leftNode.Repr := leftNode.Repr + postLeft.Repr;
-                    }
-                }
-              else
-                {
-                  if left != null
-                    {
-                      leftNode.Repr := leftNode.Repr + left.Repr;
-                      leftNode.len := left.Len();
-                    }
-                }
-
-              leftSplit := leftNode;
-
-              rightSplit := postRight;
-            }
-      }
-  }
-
-  method Concat(rope: Rope) returns (concatenatedRope: Rope)
-    requires Valid()
-    requires ValidLen()
-    requires rope.Valid()
-    requires rope.ValidLen()
-    //requires this.Repr !! rope.Repr   // prevents cycles and concatenating the same rope with itself [todo?]
-    ensures concatenatedRope.Valid()
-    ensures concatenatedRope.ValidLen()
-  {
-    concatenatedRope := new Rope.Init();
-    concatenatedRope.val := InternalNode(this, rope);
-    concatenatedRope.len := this.Len();
-    concatenatedRope.Repr := concatenatedRope.Repr + this.Repr + rope.Repr;
-  }
-
-  method Index(i: int) returns (charAtIndex: string)
-    requires Valid()
-    requires ValidLen()
-    ensures i >= 0 && this.Len() > i ==> charAtIndex != ""
-    //ensures i < 0 || this.Len() <= i ==> charAtIndex == ""
-    decreases Repr
-  {
-    match this.val
-    case Leaf(v) =>
-      if |v| <= i || i < 0
-        { charAtIndex := ""; }
-      else
-        { charAtIndex := [v[i]]; }
-    case InternalNode(left, right) =>
-      if this.len <= i
-        {
-          if right == null
-            { charAtIndex := ""; }
-          else
-            { charAtIndex := right.Index(i - this.len); }
-        }
-      else
-        {
-          if left != null
-            { charAtIndex := left.Index(i); }
-          else
-            { charAtIndex := ""; }
-        }
+    }
   }
 }
